MoonbitSemantics/Mcore/PrimTyping.lean
@@ -80,6 +80,7 @@ theorem evalPrim_type_sound'
         | unit => exact ep1_unit' heval hprim
       | unit => cases op <;> simp [evalPrim] at heval <;> simp [typeOfPrim] at hprim <;> subst_vars <;> exact .unit
       | closure => cases op <;> simp [evalPrim] at heval <;> simp [typeOfPrim] at hprim <;> subst_vars <;> first | exact .unit | exact .closure
+      | closureRec => cases op <;> simp [evalPrim] at heval <;> simp [typeOfPrim] at hprim <;> subst_vars <;> first | exact .unit | exact .closureRec
       | rawFn => cases op <;> simp [evalPrim] at heval <;> simp [typeOfPrim] at hprim <;> subst_vars <;> first | exact .unit | exact .rawFn
       | constr hvl => cases op <;> simp [evalPrim] at heval <;> simp [typeOfPrim] at hprim <;> subst_vars <;> first | exact .unit | exact .constr hvl
       | tuple hvts => cases op <;> simp [evalPrim] at heval <;> simp [typeOfPrim] at hprim <;> subst_vars <;> first | exact .unit | exact .tuple hvts
